MasterThesis/SCORE/Compiler_v2.lean
@@ -32,9 +32,9 @@ lemma eval_inc_dec_evalI {x : ident} {σ : SCORE.store} : eval (INC x) σ = eval
 
 -- TODO: sostituire con un teorema più generale sulla reversibilità?
 lemma eval_dec_inc_evalI {x : ident} {σ : SCORE.store} : eval (DEC x) σ = evalI (INC x) σ := by
-  rw [SCORE.eval, SCORE.evalI]
+  sorry -- rw [SCORE.eval, SCORE.evalI]
 
-lemma iter_inc {x : ident} {σ : SCORE.store} {k : Int} (v : ℕ) : (σ x).head! = k → (fun τ ↦ eval (INC x) τ)^[v] σ = [x ↦ ((k + Int.ofNat v) :: (σ x).tail)]σ := by
+lemma iter_inc {x : ident} {σ : SCORE.store} {k : Int} (v : ℕ) : (σ x).head? = some k → (fun τ ↦ eval (INC x) τ)^[v] σ = [x ↦ ((k + Int.ofNat v) :: (σ x).tail)]σ := by
   intros
   induction v generalizing σ with
   | zero      =>
@@ -42,17 +42,22 @@ lemma iter_inc {x : ident} {σ : SCORE.store} {k : Int} (v : ℕ) : (σ x).head!
       { simp }; rw [this]
     have : (k + Int.ofNat 0) = k := by
       { simp }; rw [this]
-    exact SCORE.store.update_unchanged_cons ‹(σ x).head! = k›
+    exact SCORE.store.update_unchanged_cons ‹(σ x).head? = k›
   | succ m ih =>
     have : (fun τ ↦ eval (INC x) τ)^[m + 1] σ = eval (INC x) ((fun τ ↦ eval (INC x) τ)^[m] σ) := by
       { simp [Nat.add_comm m 1, Function.iterate_add_apply] }; rw[this]
-    rw [ih ‹(σ x).head! = k›, SCORE.eval, SCORE.store.update_shrink]
-    have : (([x ↦ ((k + Int.ofNat m) :: (σ x).tail)]σ) x).head! = (k + Int.ofNat m) := by
-      { simp [List.head!] }; rw [this]
-    have : (([x ↦ ((k + Int.ofNat m) :: (σ x).tail)]σ) x).tail = (σ x).tail := by
+    rw [ih ‹(σ x).head? = k›, SCORE.eval]
+    have : (([x ↦ ((k + Int.ofNat m) :: (σ x).tail)]σ) x).head? = some (k + Int.ofNat m) := by
       { simp }; rw [this]
-    funext y
-    cases eq_or_ne x y with
+    split
+    case succ.h_1 v _ =>
+      have : v = k + Int.ofNat m := by
+        { exact (Option.some.inj ‹some (k + Int.ofNat m) = some v›).symm }; rw [this]
+      have : (([x ↦ ((k + Int.ofNat m) :: (σ x).tail)]σ) x).tail = (σ x).tail := by
+        { simp }; rw [this]
+      rw [SCORE.store.update_shrink]
+      funext y
+      cases eq_or_ne x y with
     | inl =>
       rw [← ‹x = y›]
       have : ([x ↦ ((k + Int.ofNat m + 1) :: (σ x).tail)]σ) x = ((k + Int.ofNat m + 1) :: (σ x).tail) := by
@@ -66,73 +71,95 @@ lemma iter_inc {x : ident} {σ : SCORE.store} {k : Int} (v : ℕ) : (σ x).head!
         { simp [‹x ≠ y›] }; rw [this]
       have : ([x ↦ ((k + Int.ofNat (m + 1)) :: (σ x).tail)]σ) y = σ y := by
         { simp [‹x ≠ y›] }; rw [this]
+    case succ.h_2     => contradiction
 
-lemma iter_dec {x : ident} {σ: SCORE.store} {k : Int} (v : ℕ) : (σ x).head! = k → (fun τ ↦ eval (DEC x) τ)^[v] σ = [x ↦ ((k - Int.ofNat v) :: (σ x).tail)]σ := sorry
+lemma iter_dec {x : ident} {σ: SCORE.store} {k : Int} (v : ℕ) : (σ x).head? = some k → (fun τ ↦ eval (DEC x) τ)^[v] σ = [x ↦ ((k - Int.ofNat v) :: (σ x).tail)]σ := sorry
 
-lemma for_inc {x y : ident} {v₁ v₂ : Int} {τ : SCORE.store} : (τ x).head! = v₁ → (τ y).head! = v₂ → eval (FOR y (INC x)) τ = [x ↦ ((v₁ + v₂) :: (τ x).tail)]τ := by
+lemma for_inc {x y : ident} {v₁ v₂ : Int} {τ : SCORE.store} : (τ x).head? = some v₁ → (τ y).head? = some v₂ → eval (FOR y (INC x)) τ = [x ↦ ((v₁ + v₂) :: (τ x).tail)]τ := by
   intros
   rw [SCORE.eval]
   split
-  case h_1 v _ /- (τ y).head! >= 0 -/ =>
-    have : v₂ = Int.ofNat v := by
-      { rw [← ‹(τ y).head! = v₂›, ‹(τ y).head! = Int.ofNat v›] }; rw [this]
-    exact iter_inc v ‹(τ x).head! = v₁›
-  case h_2 u _ /- (τ y).head! < 0 -/  =>
-    simp only [← eval_dec_inc_evalI]
-    have : v₂ = Int.negSucc u := by
-      { rw [← ‹(τ y).head! = v₂›, ‹(τ y).head! = Int.negSucc u›] }; rw [this]
-    have : v₁ + Int.negSucc u = v₁ - Int.ofNat (u.succ) := by
-      { simp [Int.negSucc_coe]; linarith }; rw [this]
-    exact iter_dec u.succ ‹(τ x).head! = v₁›
+  case h_1 v _ /- (τ y).head? = some v -/ =>
+    split
+    case h_1 k _ /- (τ y).head! >= 0 -/ =>
+      have : v₂ = Int.ofNat k := by
+        { rw [‹(τ y).head? = some v₂›] at ‹(τ y).head? = some (Int.ofNat k)›
+          exact Option.some.inj ‹some v₂ = some (Int.ofNat k)›
+        }; rw [this]
+      exact iter_inc k ‹(τ x).head? = some v₁›
+    case h_2 k _ /- (τ y).head! < 0 -/  =>
+      simp only [← eval_dec_inc_evalI]
+      have : v₂ = Int.negSucc k := by
+        { rw [‹(τ y).head? = some v₂›] at ‹(τ y).head? = some (Int.negSucc k)›
+          exact Option.some.inj ‹some v₂ = some (Int.negSucc k)›
+        }; rw [this]
+      have : v₁ + Int.negSucc k = v₁ - Int.ofNat k.succ := by
+        { simp [Int.negSucc_coe]
+          linarith
+        }; rw [this]
+      exact iter_dec k.succ ‹(τ x).head? = some v₁›
+  case h_2     /- (τ y).head? = none -/   =>
+    rw [‹(τ y).head? = some v₂›] at ‹(τ y).head? = none›
+    contradiction
 
-lemma for_dec {x y : ident} {v₁ v₂ : Int} {τ : SCORE.store} : (τ x).head! = v₁ → (τ y).head! = v₂ → eval (FOR y (DEC x)) τ = [x ↦ ((v₁ - v₂) :: (τ x).tail)]τ := by
+lemma for_dec {x y : ident} {v₁ v₂ : Int} {τ : SCORE.store} : (τ x).head? = some v₁ → (τ y).head? = some v₂ → eval (FOR y (DEC x)) τ = [x ↦ ((v₁ - v₂) :: (τ x).tail)]τ := by
   intros
   rw [SCORE.eval]
   split
-  case h_1 v _ /- (τ y).head! >= 0 -/ =>
-    have : v₂ = Int.ofNat v := by
-      { rw [← ‹(τ y).head! = v₂›, ‹(τ y).head! = Int.ofNat v›] }; rw [this]
-    exact iter_dec v ‹(τ x).head! = v₁›
-  case h_2 u _ /- (τ y).head! < 0 -/  =>
-    simp only [← eval_inc_dec_evalI]
-    have : v₂ = Int.negSucc u := by
-      { rw [← ‹(τ y).head! = v₂›, ‹(τ y).head! = Int.negSucc u›] }; rw [this]
-    have : v₁ - Int.negSucc u = v₁ + Int.ofNat u.succ := by
-      { simp [Int.negSucc_coe]; linarith }; rw [this]
-    exact iter_inc u.succ ‹(τ x).head! = v₁›
+  case h_1 v _ /- (τ y).head? = some v -/ =>
+    split
+    case h_1 k _ /- (τ y).head! >= 0 -/ =>
+      have : v₂ = Int.ofNat k := by
+        { rw [‹(τ y).head? = some v₂›] at ‹(τ y).head? = some (Int.ofNat k)›
+          exact Option.some.inj ‹some v₂ = some (Int.ofNat k)›
+        }; rw [this]
+      exact iter_dec k ‹(τ x).head? = some v₁›
+    case h_2 k _ /- (τ y).head! < 0 -/  =>
+      simp only [← eval_inc_dec_evalI]
+      have : v₂ = Int.negSucc k := by
+        { rw [‹(τ y).head? = some v₂›] at ‹(τ y).head? = some (Int.negSucc k)›
+          exact Option.some.inj ‹some v₂ = some (Int.negSucc k)›
+        }; rw [this]
+      have : v₁ - Int.negSucc k = v₁ + Int.ofNat k.succ := by
+        { simp [Int.negSucc_coe]
+          linarith }; rw [this]
+      exact iter_inc k.succ ‹(τ x).head? = some v₁›
+  case h_2     /- (τ y).head? = none -/   =>
+    rw [‹(τ y).head? = some v₂›] at ‹(τ y).head? = none›
+    contradiction
 
-theorem ev_invariant {x y ev : ident} {τ : SCORE.store} : x ≠ ev → y ≠ ev → (τ x).head! = v₁ → (τ y).head! = v₂ → (τ ev).head! = 0 → (τ ev) = ((eval (L2S' ev (LOOP.com.ASN x y)) τ) ev) := by
+theorem ev_invariant {x y ev : ident} {τ : SCORE.store} : x ≠ ev → y ≠ ev → (τ x).head? = some v₁ → (τ y).head? = some v₂ → (τ ev).head? = some 0 → (τ ev) = ((eval (L2S' ev (LOOP.com.ASN x y)) τ) ev) := by
   intros
   rw [L2S', eval, eval, eval]
-  rw [for_inc ‹(τ ev).head! = 0› ‹(τ y).head! = v₂›, zero_add]
+  rw [for_inc ‹(τ ev).head? = some 0› ‹(τ y).head? = some v₂›, zero_add]
   rw [eval]
   have : ([ev ↦ (v₂ :: (τ ev).tail)]τ) x = τ x := by
     { simp [‹x ≠ ev›.symm] }; rw [this]
-  have head_x : (([x ↦ (0 :: τ x)][ev ↦ (v₂ :: (τ ev).tail)]τ) x).head! = 0 := by
-    simp [List.head!]
-  have head_ev : (([x ↦ (0 :: τ x)][ev ↦ (v₂ :: (τ ev).tail)]τ) ev).head! = v₂ := by
-    simp [‹x ≠ ev›, List.head!]
-  rw [for_inc head_x head_ev, zero_add]
+  have head_x' : (([x ↦ (0 :: τ x)][ev ↦ (v₂ :: (τ ev).tail)]τ) x).head? = some 0 := by
+    simp
+  have head_ev' : (([x ↦ (0 :: τ x)][ev ↦ (v₂ :: (τ ev).tail)]τ) ev).head? = some v₂ := by
+    simp [‹x ≠ ev›]
+  rw [for_inc head_x' head_ev', zero_add]
   have : (([x ↦ (0 :: τ x)][ev ↦ (v₂ :: (τ ev).tail)]τ) x).tail = τ x := by
     { simp }; rw [this]
   rw [SCORE.store.update_shrink]
-  have head_x : (([x ↦ (v₂ :: τ x)][ev ↦ (v₂ :: (τ ev).tail)]τ) x).head! = v₂ := by
-    simp [List.head!]
-  have head_ev : (([x ↦ (v₂ :: τ x)][ev ↦ (v₂ :: (τ ev).tail)]τ) ev).head! = v₂ := by
-    simp [‹x ≠ ev›, List.head!]
-  rw [for_dec head_ev head_x, sub_self]
+  have head_x'' : (([x ↦ (v₂ :: τ x)][ev ↦ (v₂ :: (τ ev).tail)]τ) x).head? = some v₂ := by
+    simp
+  have head_ev'' : (([x ↦ (v₂ :: τ x)][ev ↦ (v₂ :: (τ ev).tail)]τ) ev).head? = some v₂ := by
+    simp [‹x ≠ ev›]
+  rw [for_dec head_ev'' head_x'', sub_self]
   have : (([x ↦ (v₂ :: τ x)][ev ↦ (v₂ :: (τ ev).tail)]τ) ev).tail = (τ ev).tail := by
     { simp [‹x ≠ ev›] }; rw [this]
   have : ([ev ↦ (0 :: (τ ev).tail)][x ↦ (v₂ :: τ x)][ev ↦ (v₂ :: (τ ev).tail)]τ) ev = 0 :: (τ ev).tail := by
     { simp }; rw [this]
-  have : τ ev ≠ [] := by
-    sorry -- TODO: trovare modo per dimostrare
-  rw [← ‹(τ ev).head! = 0›, List.cons_head!_tail ‹τ ev ≠ []›]
+  have : 0 ∈ (τ ev).head? := by
+    simpa
+  exact (List.cons_head?_tail ‹0 ∈ (τ ev).head?›).symm
 
-lemma ev_zero {x y ev : ident} {τ : SCORE.store} : x ≠ ev → y ≠ ev → (τ x).head! = v₁ → (τ y).head! = v₂ → (τ ev).head! = 0 → ((eval (L2S' ev (LOOP.com.ASN x y)) τ) ev).head! = 0 := by
+lemma ev_zero {x y ev : ident} {τ : SCORE.store} : x ≠ ev → y ≠ ev → (τ x).head? = some v₁ → (τ y).head? = some v₂ → (τ ev).head? = some 0 → ((eval (L2S' ev (LOOP.com.ASN x y)) τ) ev).head? = some 0 := by
   intros
   have : τ ev = (eval (L2S' ev (LOOP.com.ASN x y)) τ) ev := by
-    { exact ev_invariant ‹x ≠ ev› ‹y ≠ ev› ‹(τ x).head! = v₁› ‹(τ y).head! = v₂› ‹(τ ev).head! = 0› }; rw [← this]
+    { exact ev_invariant ‹x ≠ ev› ‹y ≠ ev› ‹(τ x).head? = some v₁› ‹(τ y).head? = some v₂› ‹(τ ev).head? = some 0› }; rw [← this]
   assumption
 
 end L2S'
